@prefix cs:     <https://www.opengis.net/def/ogc-api/records> .
@prefix rec:    <https://www.opengis.net/def/ogc-api/records/> .

@prefix rdfs:   <http://www.w3.org/2000/01/rdf-schema#>.
@prefix dct:    <http://purl.org/dc/terms/>.
@prefix skos:   <http://www.w3.org/2004/02/skos/core#> .
@prefix owl:    <http://www.w3.org/2002/07/owl#>.
@prefix xsd:    <http://www.w3.org/2001/XMLSchema#>.
@prefix schema: <http://schema.org/>.

cs:
    a              skos:ConceptScheme ;
    skos:prefLabel "OGC API Records" .

rec:hasLinkTemplate
    a              skos:Concept, owl:ObjectProperty ;
    skos:inScheme  cs: ;
    skos:prefLabel "has link template" ;
    skos:definition """"a link template based on the schema for a link that includes substitution variables who’s values are filled in at runtime prior to resolving the link.

Information about the substitution variables can be obtained in one of two ways. The variable property may be used to encode the definitions of substitution variables in-line in the link. Alternatively, the varBase property can be used to specify a base URI to which a variable name may be appended to retrieve the definition of the specified substitution variable.""" ;
    rdfs:range     rec:LinkTemplate ;
.

rec:LinkTemplate
    a              skos:Concept, owl:Class ;
    skos:prefLabel "Link template" ;
    skos:definition """"a link template based on the schema for a link that includes substitution variables who’s values are filled in at runtime prior to resolving the link.

Information about the substitution variables can be obtained in one of two ways. The variable property may be used to encode the definitions of substitution variables in-line in the link. Alternatively, the varBase property can be used to specify a base URI to which a variable name may be appended to retrieve the definition of the specified substitution variable.""" ;
    skos:inScheme  cs: ;
.

rec:uriTemplate
    a               skos:Concept, owl:DatatypeProperty ;
    skos:prefLabel  "URI template" ;
    skos:definition "Supplies a resolvable URI to a remote resource (or resource fragment)." ;
    skos:inScheme   cs: ;
    rdfs:domain     rec:linkTemplate ;
    rdfs:range      xsd:string ;
.

rec:varBase
    a              skos:Concept, owl:DatatypeProperty ;
    skos:prefLabel "variable base" ;
    skos:definition
                   "The base URI to which a variable name can be appended to retrieve the definition of the variable as a JSON Schema fragment." ;
    skos:inScheme  cs: ;
    rdfs:domain    rec:linkTemplate ;
    rdfs:range     xsd:string ;
.

rec:hasVariable
    a              skos:Concept, owl:ObjectProperty ;
    skos:prefLabel "has variable" ;
    skos:definition """"a substitution variable in the associated linkTemplate""" ;
    skos:inScheme  cs: ;
    rdfs:domain    rec:linkTemplate ;
    rdfs:range     rec:LinkTemplateVariable ;
.

rec:LinkTemplateVariable
    a               skos:Concept, owl:Class ;
    skos:prefLabel  "Link Template Variable" ;
    skos:inScheme   cs: ;
    skos:definition """"a substitution variable in the associated linkTemplate""" ;
    # Require dct:identifier for the variable
    rdfs:subClassOf [ a               owl:Restriction ;
                      owl:cardinality 1 ;
                      owl:onProperty  dct:identifier ; ] ;

    # JSON Schema provided in dct:format
    rdfs:subClassOf [ a                           owl:Restriction ;
                      owl:qualifiedMinCardinality 1 ;
                      owl:onProperty              dct:format ;
                      owl:onClass                 <https://www.w3.org/2019/wot/json-schema#DataSchema> ; ] ;
.

rec:iso8601period
    a               skos:Concept, owl:DatatypeProperty ;
    skos:prefLabel  "TimePeriod" ;
    skos:definition "A Time period expressed in ISO 8601 notation - such as P1D" ;
    rdfs:range      xsd:string ;
    skos:inScheme   cs: ;
.

rec:scheme
    a               skos:Concept, owl:DatatypeProperty ;
    skos:prefLabel  "Id scheme" ;
    skos:definition """A reference to an authority or identifier for a knowledge organization system from which the external identifier was obtained. It is recommended that the identifier be a resolvable URI.""" ;
    rdfs:range      xsd:string ;
    skos:inScheme   cs: ;
.

rec:value
    a               skos:Concept, owl:DatatypeProperty ;
    skos:prefLabel  "Identifier" ;
    skos:definition """The value of the identifier""" ;
    rdfs:range      xsd:string ;
    skos:inScheme   cs: ;
.

rec:format
    a               skos:Concept, owl:DatatypeProperty ;
    skos:prefLabel  "Available Format" ;
    skos:definition """Available distributions of the resource""" ;
    rdfs:range      xsd:string ;
    skos:inScheme   cs: ;
.

