@prefix cs: <https://www.opengis.net/def/ogc-api/records> .
@prefix dct: <http://purl.org/dc/terms/> .
@prefix owl: <http://www.w3.org/2002/07/owl#> .
@prefix rdfs: <http://www.w3.org/2000/01/rdf-schema#> .
@prefix rec: <https://www.opengis.net/def/ogc-api/records/> .
@prefix skos: <http://www.w3.org/2004/02/skos/core#> .
@prefix xsd: <http://www.w3.org/2001/XMLSchema#> .

rec:format a owl:DatatypeProperty,
        skos:Concept ;
    rdfs:range xsd:string ;
    skos:definition "Available distributions of the resource" ;
    skos:inScheme cs: ;
    skos:prefLabel "Available Format" .

rec:hasLinkTemplate a owl:ObjectProperty,
        skos:Concept ;
    rdfs:range rec:LinkTemplate ;
    skos:definition """"a link template based on the schema for a link that includes substitution variables who’s values are filled in at runtime prior to resolving the link.

Information about the substitution variables can be obtained in one of two ways. The variable property may be used to encode the definitions of substitution variables in-line in the link. Alternatively, the varBase property can be used to specify a base URI to which a variable name may be appended to retrieve the definition of the specified substitution variable.""" ;
    skos:inScheme cs: ;
    skos:prefLabel "has link template" .

rec:hasVariable a owl:ObjectProperty,
        skos:Concept ;
    rdfs:domain rec:linkTemplate ;
    rdfs:range rec:LinkTemplateVariable ;
    skos:definition "\"a substitution variable in the associated linkTemplate" ;
    skos:inScheme cs: ;
    skos:prefLabel "has variable" .

rec:iso8601period a owl:DatatypeProperty,
        skos:Concept ;
    rdfs:range xsd:string ;
    skos:definition "A Time period expressed in ISO 8601 notation - such as P1D" ;
    skos:inScheme cs: ;
    skos:prefLabel "TimePeriod" .

rec:scheme a owl:DatatypeProperty,
        skos:Concept ;
    rdfs:range xsd:string ;
    skos:definition "A reference to an authority or identifier for a knowledge organization system from which the external identifier was obtained. It is recommended that the identifier be a resolvable URI." ;
    skos:inScheme cs: ;
    skos:prefLabel "Id scheme" .

rec:uriTemplate a owl:DatatypeProperty,
        skos:Concept ;
    rdfs:domain rec:linkTemplate ;
    rdfs:range xsd:string ;
    skos:definition "Supplies a resolvable URI to a remote resource (or resource fragment)." ;
    skos:inScheme cs: ;
    skos:prefLabel "URI template" .

rec:value a owl:DatatypeProperty,
        skos:Concept ;
    rdfs:range xsd:string ;
    skos:definition "The value of the identifier" ;
    skos:inScheme cs: ;
    skos:prefLabel "Identifier" .

rec:varBase a owl:DatatypeProperty,
        skos:Concept ;
    rdfs:domain rec:linkTemplate ;
    rdfs:range xsd:string ;
    skos:definition "The base URI to which a variable name can be appended to retrieve the definition of the variable as a JSON Schema fragment." ;
    skos:inScheme cs: ;
    skos:prefLabel "variable base" .

rec:LinkTemplate a owl:Class,
        skos:Concept ;
    skos:definition """"a link template based on the schema for a link that includes substitution variables who’s values are filled in at runtime prior to resolving the link.

Information about the substitution variables can be obtained in one of two ways. The variable property may be used to encode the definitions of substitution variables in-line in the link. Alternatively, the varBase property can be used to specify a base URI to which a variable name may be appended to retrieve the definition of the specified substitution variable.""" ;
    skos:inScheme cs: ;
    skos:prefLabel "Link template" .

rec:LinkTemplateVariable a owl:Class,
        skos:Concept ;
    rdfs:subClassOf [ a owl:Restriction ;
            owl:cardinality 1 ;
            owl:onProperty dct:identifier ],
        [ a owl:Restriction ;
            owl:onClass <https://www.w3.org/2019/wot/json-schema#DataSchema> ;
            owl:onProperty dct:format ;
            owl:qualifiedMinCardinality 1 ] ;
    skos:definition "\"a substitution variable in the associated linkTemplate" ;
    skos:inScheme cs: ;
    skos:prefLabel "Link Template Variable" .

cs: a skos:ConceptScheme ;
    skos:prefLabel "OGC API Records" .

